@prefix biolink: <https://w3id.org/biolink/vocab/> .
@prefix dcterms: <http://purl.org/dc/terms/> .
@prefix linkml: <https://w3id.org/linkml/> .
@prefix owl: <http://www.w3.org/2002/07/owl#> .
@prefix pav: <http://purl.org/pav/> .
@prefix rdfs: <http://www.w3.org/2000/01/rdf-schema#> .
@prefix skos: <http://www.w3.org/2004/02/skos/core#> .
@prefix xsd: <http://www.w3.org/2001/XMLSchema#> .

biolink:IngestMetadataFile a owl:Class,
        linkml:ClassDefinition ;
    rdfs:label "IngestMetadataFile" ;
    rdfs:subClassOf [ a owl:Restriction ;
            owl:allValuesFrom linkml:String ;
            owl:onProperty biolink:file_created_by ],
        [ a owl:Restriction ;
            owl:maxCardinality 1 ;
            owl:onProperty biolink:node_normalizer_url ],
        [ a owl:Restriction ;
            owl:allValuesFrom linkml:String ;
            owl:onProperty biolink:source_data_version ],
        [ a owl:Restriction ;
            owl:maxCardinality 1 ;
            owl:onProperty biolink:node_normalizer_version ],
        [ a owl:Restriction ;
            owl:minCardinality 1 ;
            owl:onProperty biolink:target_format ],
        [ a owl:Restriction ;
            owl:minCardinality 0 ;
            owl:onProperty biolink:edge_predicates ],
        [ a owl:Restriction ;
            owl:maxCardinality 1 ;
            owl:onProperty biolink:source_access_date ],
        [ a owl:Restriction ;
            owl:allValuesFrom linkml:String ;
            owl:onProperty biolink:target_name ],
        [ a owl:Restriction ;
            owl:allValuesFrom linkml:Date ;
            owl:onProperty biolink:target_creation_date ],
        [ a owl:Restriction ;
            owl:minCardinality 1 ;
            owl:onProperty biolink:target_data_model_version ],
        [ a owl:Restriction ;
            owl:maxCardinality 1 ;
            owl:onProperty biolink:orphan_node_count ],
        [ a owl:Restriction ;
            owl:maxCardinality 1 ;
            owl:onProperty biolink:total_node_count ],
        [ a owl:Restriction ;
            owl:allValuesFrom linkml:Integer ;
            owl:onProperty biolink:orphan_node_count ],
        [ a owl:Restriction ;
            owl:allValuesFrom linkml:Date ;
            owl:onProperty biolink:file_creation_date ],
        [ a owl:Restriction ;
            owl:minCardinality 0 ;
            owl:onProperty biolink:source_file_names ],
        [ a owl:Restriction ;
            owl:allValuesFrom linkml:Integer ;
            owl:onProperty biolink:total_node_count ],
        [ a owl:Restriction ;
            owl:minCardinality 1 ;
            owl:onProperty biolink:source_data_version ],
        [ a owl:Restriction ;
            owl:allValuesFrom linkml:String ;
            owl:onProperty biolink:target_model_url ],
        [ a owl:Restriction ;
            owl:maxCardinality 1 ;
            owl:onProperty biolink:target_data_model_version ],
        [ a owl:Restriction ;
            owl:allValuesFrom linkml:String ;
            owl:onProperty biolink:source_file_names ],
        [ a owl:Restriction ;
            owl:minCardinality 1 ;
            owl:onProperty biolink:target_model ],
        [ a owl:Restriction ;
            owl:allValuesFrom linkml:String ;
            owl:onProperty biolink:node_normalizer_url ],
        [ a owl:Restriction ;
            owl:allValuesFrom linkml:Uriorcurie ;
            owl:onProperty biolink:source_access_urls ],
        [ a owl:Restriction ;
            owl:allValuesFrom linkml:String ;
            owl:onProperty biolink:edge_predicates ],
        [ a owl:Restriction ;
            owl:allValuesFrom linkml:String ;
            owl:onProperty biolink:node_categories ],
        [ a owl:Restriction ;
            owl:minCardinality 0 ;
            owl:onProperty biolink:total_node_count ],
        [ a owl:Restriction ;
            owl:allValuesFrom linkml:String ;
            owl:onProperty biolink:ingest_code_version ],
        [ a owl:Restriction ;
            owl:maxCardinality 1 ;
            owl:onProperty biolink:total_edge_count ],
        [ a owl:Restriction ;
            owl:minCardinality 1 ;
            owl:onProperty biolink:file_creation_date ],
        [ a owl:Restriction ;
            owl:allValuesFrom linkml:Uriorcurie ;
            owl:onProperty biolink:ingest_code_url ],
        [ a owl:Restriction ;
            owl:minCardinality 1 ;
            owl:onProperty biolink:file_name ],
        [ a owl:Restriction ;
            owl:maxCardinality 1 ;
            owl:onProperty biolink:target_model_url ],
        [ a owl:Restriction ;
            owl:allValuesFrom linkml:String ;
            owl:onProperty biolink:node_normalizer ],
        [ a owl:Restriction ;
            owl:allValuesFrom linkml:String ;
            owl:onProperty biolink:node_normalizer_version ],
        [ a owl:Restriction ;
            owl:maxCardinality 1 ;
            owl:onProperty biolink:file_name ],
        [ a owl:Restriction ;
            owl:maxCardinality 1 ;
            owl:onProperty biolink:ingest_code_url ],
        [ a owl:Restriction ;
            owl:allValuesFrom linkml:Integer ;
            owl:onProperty biolink:total_edge_count ],
        [ a owl:Restriction ;
            owl:maxCardinality 1 ;
            owl:onProperty biolink:source_data_version ],
        [ a owl:Restriction ;
            owl:minCardinality 0 ;
            owl:onProperty biolink:node_categories ],
        [ a owl:Restriction ;
            owl:minCardinality 1 ;
            owl:onProperty biolink:target_creation_date ],
        [ a owl:Restriction ;
            owl:minCardinality 0 ;
            owl:onProperty biolink:node_normalizer ],
        [ a owl:Restriction ;
            owl:maxCardinality 1 ;
            owl:onProperty biolink:node_normalizer ],
        [ a owl:Restriction ;
            owl:allValuesFrom linkml:String ;
            owl:onProperty biolink:target_format ],
        [ a owl:Restriction ;
            owl:minCardinality 0 ;
            owl:onProperty biolink:orphan_node_count ],
        [ a owl:Restriction ;
            owl:maxCardinality 1 ;
            owl:onProperty biolink:target_creation_date ],
        [ a owl:Restriction ;
            owl:maxCardinality 1 ;
            owl:onProperty biolink:target_format ],
        [ a owl:Restriction ;
            owl:allValuesFrom linkml:String ;
            owl:onProperty biolink:file_name ],
        [ a owl:Restriction ;
            owl:minCardinality 0 ;
            owl:onProperty biolink:target_model_url ],
        [ a owl:Restriction ;
            owl:maxCardinality 1 ;
            owl:onProperty biolink:source_infores_id ],
        [ a owl:Restriction ;
            owl:minCardinality 0 ;
            owl:onProperty biolink:source_access_urls ],
        [ a owl:Restriction ;
            owl:minCardinality 1 ;
            owl:onProperty biolink:target_name ],
        [ a owl:Restriction ;
            owl:minCardinality 1 ;
            owl:onProperty biolink:source_access_date ],
        [ a owl:Restriction ;
            owl:allValuesFrom linkml:Date ;
            owl:onProperty biolink:source_access_date ],
        [ a owl:Restriction ;
            owl:maxCardinality 1 ;
            owl:onProperty biolink:file_creation_date ],
        [ a owl:Restriction ;
            owl:minCardinality 0 ;
            owl:onProperty biolink:node_normalizer_version ],
        [ a owl:Restriction ;
            owl:maxCardinality 1 ;
            owl:onProperty biolink:target_model ],
        [ a owl:Restriction ;
            owl:minCardinality 0 ;
            owl:onProperty biolink:total_edge_count ],
        [ a owl:Restriction ;
            owl:maxCardinality 1 ;
            owl:onProperty biolink:ingest_code_version ],
        [ a owl:Restriction ;
            owl:minCardinality 1 ;
            owl:onProperty biolink:ingest_code_url ],
        [ a owl:Restriction ;
            owl:minCardinality 1 ;
            owl:onProperty biolink:ingest_code_version ],
        [ a owl:Restriction ;
            owl:minCardinality 0 ;
            owl:onProperty biolink:file_created_by ],
        [ a owl:Restriction ;
            owl:allValuesFrom linkml:String ;
            owl:onProperty biolink:target_data_model_version ],
        [ a owl:Restriction ;
            owl:allValuesFrom linkml:String ;
            owl:onProperty biolink:target_model ],
        [ a owl:Restriction ;
            owl:minCardinality 1 ;
            owl:onProperty biolink:source_infores_id ],
        [ a owl:Restriction ;
            owl:allValuesFrom linkml:Uriorcurie ;
            owl:onProperty biolink:source_infores_id ],
        [ a owl:Restriction ;
            owl:maxCardinality 1 ;
            owl:onProperty biolink:target_name ],
        [ a owl:Restriction ;
            owl:minCardinality 0 ;
            owl:onProperty biolink:node_normalizer_url ] ;
    skos:definition """Information about a particular ingest performed to produce a KGX graph, describing source data, ingest process, and details of the resulting KGX graph.
""" ;
    skos:inScheme <https://w3id.org/biolink/kgx/ingest-metadata-schema> .

biolink:edge_predicates a owl:ObjectProperty,
        linkml:SlotDefinition ;
    rdfs:label "edge_predicates" ;
    skos:definition "List of all Biolink predicates used in the graph." ;
    skos:inScheme <https://w3id.org/biolink/kgx/ingest-metadata-schema> .

biolink:file_created_by a owl:ObjectProperty,
        linkml:SlotDefinition ;
    rdfs:label "file_created_by" ;
    skos:definition """The agent(s) (person if hand-authored, software tool if created programmatically) that created this ingest metadata file.
""" ;
    skos:inScheme <https://w3id.org/biolink/kgx/ingest-metadata-schema> .

biolink:node_categories a owl:ObjectProperty,
        linkml:SlotDefinition ;
    rdfs:label "node_categories" ;
    skos:definition "List of all Biolink categories used for nodes in the graph." ;
    skos:inScheme <https://w3id.org/biolink/kgx/ingest-metadata-schema> .

biolink:source_access_urls a owl:ObjectProperty,
        linkml:SlotDefinition ;
    rdfs:label "source_access_urls" ;
    skos:definition """URLs where source data was accessed / downloaded / queried to be brought into the system performing the ingest.
""" ;
    skos:inScheme <https://w3id.org/biolink/kgx/ingest-metadata-schema> .

biolink:source_file_names a owl:ObjectProperty,
        linkml:SlotDefinition ;
    rdfs:label "source_file_names" ;
    skos:definition """File names from which content used to produce the output KGX graph was retrieved.
""" ;
    skos:inScheme <https://w3id.org/biolink/kgx/ingest-metadata-schema> .

biolink:file_creation_date a owl:ObjectProperty,
        linkml:SlotDefinition ;
    rdfs:label "file_creation_date" ;
    skos:definition "When this metadata file was created." ;
    skos:inScheme <https://w3id.org/biolink/kgx/ingest-metadata-schema> .

biolink:file_name a owl:ObjectProperty,
        linkml:SlotDefinition ;
    rdfs:label "file_name" ;
    skos:definition """An informative, human-readable name for this metadata file/object. e.g. "2025-08-18 Translator CTD Ingest Metadata"
""" ;
    skos:inScheme <https://w3id.org/biolink/kgx/ingest-metadata-schema> .

biolink:ingest_code_url a owl:ObjectProperty,
        linkml:SlotDefinition ;
    rdfs:label "ingest_code_url" ;
    skos:definition """URL of the specific official release or tagged branch of the ingest code executed to perform the ingest.
""" ;
    skos:inScheme <https://w3id.org/biolink/kgx/ingest-metadata-schema> .

biolink:ingest_code_version a owl:ObjectProperty,
        linkml:SlotDefinition ;
    rdfs:label "ingest_code_version" ;
    skos:definition """The version of the ingest code executed to perform the ingest.
""" ;
    skos:inScheme <https://w3id.org/biolink/kgx/ingest-metadata-schema> .

biolink:node_normalizer a owl:ObjectProperty,
        linkml:SlotDefinition ;
    rdfs:label "node_normalizer" ;
    skos:definition """Name/identifier of the algorithm/tool used to perform node normalization on the ingested data. e.g. "Babel"
""" ;
    skos:inScheme <https://w3id.org/biolink/kgx/ingest-metadata-schema> .

biolink:node_normalizer_url a owl:ObjectProperty,
        linkml:SlotDefinition ;
    rdfs:label "node_normalizer_url" ;
    skos:definition """URL(s) pointing to source code and/or information about the node normalization tool used. e.g. "https://github.com/TranslatorSRI/NodeNormalization"
""" ;
    skos:inScheme <https://w3id.org/biolink/kgx/ingest-metadata-schema> .

biolink:node_normalizer_version a owl:ObjectProperty,
        linkml:SlotDefinition ;
    rdfs:label "node_normalizer_version" ;
    skos:definition "Version of the node normalization tool/algorithm." ;
    skos:inScheme <https://w3id.org/biolink/kgx/ingest-metadata-schema> .

biolink:orphan_node_count a owl:ObjectProperty,
        linkml:SlotDefinition ;
    rdfs:label "orphan_node_count" ;
    skos:definition """Count of nodes in the graph that do not participate in an edge.
""" ;
    skos:inScheme <https://w3id.org/biolink/kgx/ingest-metadata-schema> .

biolink:source_access_date a owl:ObjectProperty,
        linkml:SlotDefinition ;
    rdfs:label "source_access_date" ;
    skos:definition """Date the source data was accessed/downloaded into the system that performed the ingest.
""" ;
    skos:inScheme <https://w3id.org/biolink/kgx/ingest-metadata-schema> .

biolink:source_data_version a owl:ObjectProperty,
        linkml:SlotDefinition ;
    rdfs:label "source_data_version" ;
    skos:definition """Version of the source data ingested - using source's own conventions, or make one up (e.g. use the date) if not provided by source.
""" ;
    skos:inScheme <https://w3id.org/biolink/kgx/ingest-metadata-schema> .

biolink:source_infores_id a owl:ObjectProperty,
        linkml:SlotDefinition ;
    rdfs:label "source_infores_id" ;
    skos:definition "Infores identifier of the ingested source." ;
    skos:inScheme <https://w3id.org/biolink/kgx/ingest-metadata-schema> .

biolink:target_creation_date a owl:ObjectProperty,
        linkml:SlotDefinition ;
    rdfs:label "target_creation_date" ;
    skos:definition "Date the target data set/graph was created." ;
    skos:inScheme <https://w3id.org/biolink/kgx/ingest-metadata-schema> .

biolink:target_data_model_version a owl:ObjectProperty,
        linkml:SlotDefinition ;
    rdfs:label "target_data_model_version" ;
    skos:definition """Version of the target data model used to structure the KGX graph data. e.g. "4.2.6-rc5"
""" ;
    skos:inScheme <https://w3id.org/biolink/kgx/ingest-metadata-schema> .

biolink:target_format a owl:ObjectProperty,
        linkml:SlotDefinition ;
    rdfs:label "target_format" ;
    skos:definition """Format in which the KGX graph is serialized (e.g., "KGX-jsonlines").
""" ;
    skos:inScheme <https://w3id.org/biolink/kgx/ingest-metadata-schema> .

biolink:target_model a owl:ObjectProperty,
        linkml:SlotDefinition ;
    rdfs:label "target_model" ;
    skos:definition """Name/identifier of the data model used to structure the KGX graph data.
""" ;
    skos:inScheme <https://w3id.org/biolink/kgx/ingest-metadata-schema> ;
    skos:note "This will be Biolink Model for all Translator graphs - which can be referenced as \"https://w3id.org/biolink/biolink-model\"" .

biolink:target_model_url a owl:ObjectProperty,
        linkml:SlotDefinition ;
    rdfs:label "target_model_url" ;
    skos:definition """A URL providing information about the data model used to structure the KGX graph data. e.g. "https://biolink.github.io/biolink-model/"
""" ;
    skos:inScheme <https://w3id.org/biolink/kgx/ingest-metadata-schema> .

biolink:target_name a owl:ObjectProperty,
        linkml:SlotDefinition ;
    rdfs:label "target_name" ;
    skos:definition """A unique human readable name of the target data set/graph produced by this ingest. e.g. "2025-08-18 Translator CTD Ingest Graph"
""" ;
    skos:inScheme <https://w3id.org/biolink/kgx/ingest-metadata-schema> .

biolink:total_edge_count a owl:ObjectProperty,
        linkml:SlotDefinition ;
    rdfs:label "total_edge_count" ;
    skos:definition "Count of total edges in the graph." ;
    skos:inScheme <https://w3id.org/biolink/kgx/ingest-metadata-schema> .

biolink:total_node_count a owl:ObjectProperty,
        linkml:SlotDefinition ;
    rdfs:label "total_node_count" ;
    skos:definition "Count of total nodes in the graph." ;
    skos:inScheme <https://w3id.org/biolink/kgx/ingest-metadata-schema> .

<https://w3id.org/biolink/kgx/ingest-metadata-schema> a owl:Ontology ;
    rdfs:label "kgx_ingest_metadata_schema" ;
    dcterms:license "https://creativecommons.org/publicdomain/zero/1.0/" ;
    dcterms:title "KGX Ingest Metadata Schema" ;
    pav:version "0.1.0" ;
    skos:definition "A schema for describing metadata about a specific execution of a source ingest to produce a specific KGX-format graph." ;
    skos:note """- An ingest metadata file holds information about a specific execution
  of an ingest of a given source - of which there may be many over time,
  to produce different instances KGX outputs.
- A RIG describes more general specification and rationale for ingesting
  a given source, that is mean to apply across any specific ingest execution.
- Content of these two descriptive artifacts is intended to be
  complementary / non-overlapping.""" .

